\section*{Appendix I: On Phase Singularities}

To construct the expression for an isolated optical vortex, we start from the wave equation
\begin{eqnarray}
	&&c^2\nabla^2\psi = \frac{\partial^2 \psi}{\partial t^2}.
	\label{eq:wave}
\end{eqnarray}
One can verify that wave functions of the form
\begin{eqnarray}
	&&\psi = (a + b\textcolor{blue}{y}) e^{i(kz - \omega t)}
	\label{eqn_301}
\end{eqnarray}
which are waves with linearly modulated amplitude, satisfy Eq. (\ref{eq:wave}). 
Now we consider two primary wave trains, say wave $A$ and $B$, assuming that they are monochromatic and modulated linearly along $y$-direction so that one rises, as the other falls. 
If wave $A$ and $B$ coincide with each other on the $y = 0$ plane with an angle $2 \alpha$ (see Fig. \ref{fig:two_primary_waves}), one can write down their wave expression
\begin{eqnarray}
	&&\psi_A = a_0(1 + \beta k_1 y) e^{i(k_1 x + k_3 z - \omega t - \pi/2)}
	\nonumber \\
	&&\psi_B = a_0(1 - \beta k_1 y) e^{i(-k_1 x + k_3 z - \omega t + \pi/2)}
	\label{eqn_302}
\end{eqnarray}
\textcolor{red}{Draw a schematic to represent $\psi_A$ and $\psi_B$.
	Resosolve the inconsistency between $\psi_A$, $\psi_B$ in (\ref{eqn_302}) and $\psi$ in (\ref{eqn_301}).}
where $\bar{k} = \hat{x} k_1 + \hat{z} k_3$ is the propagating vector of wave $A$, 
$a_0$ and $\beta$ are constants representing the amplitudes of carrier and modulating waves, respectively.

% Unable to show figure?
%\begin{figure}[h]
%	\vskip 6 cm
%	\hskip 0.3 cm
%	\special{wmf: primary_waves.pdf x=7 cm y=6 cm}
%	\caption{Illustration for the primary waves $A$ and $B$.}
%	\label{fig:two_primary_waves}
%\end{figure}
\begin{figure}[h]
	\centering
	\includegraphics[width = 0.4\textwidth]{primary_waves.jpg}
	\caption{Illustration for the primary waves $A$ and $B$.}
	\label{fig:two_primary_waves}
\end{figure}

Let $c = \omega/k$, $k_1 = k \sin \alpha$, $k_3 = k \cos \alpha$, $\xi = k_1 x$, $\zeta = k_3 z - \omega t$ and $\eta = k_1 y$. 
The resultant complex wave field can be represented by the superposition of $A$ and $B$,
\begin{eqnarray}
	&&\psi = \psi_A + \psi_B = a_0 \left[ ( 1 + \beta \eta ) e^{i(\xi + \zeta - \pi/2)} \right. 
	\nonumber\\
	&&\hspace{0.3in} \left. + ( 1 - \beta \eta ) e^{i (- \xi + \zeta + \pi/2)} \right]
	\nonumber\\
	&&= 2 a_0 e^{i\zeta} \left[ \cos(\xi - \pi/2) + i \beta \eta \sin(\xi - \pi/2) \right]
	\nonumber\\
	&&= 2 a_0 e^{i\zeta} \left( \sin \xi - i \beta \eta \cos\xi \right)
	\nonumber
\end{eqnarray}
Therefore we can explicitly write down the formula of the wave in complex forms, \textcolor{blue}{$\psi = |\psi| e^{i\Phi}$,}
\textcolor{red}{What are $\rho$ and $\Phi$?}
\begin{eqnarray}
	&&\textcolor{blue}{|\psi|^2} = 4a_0^2 (\sin^2 \xi + \beta^2 \eta^2 \cos^2 \xi)
	\nonumber\\
	&&\Phi = 2n\pi + \zeta - \arctan\left(\frac{\beta \eta}{\tan \xi} \right).
\end{eqnarray}
Now, put $A_0 = 2a_0 \sin\alpha$ and let $\alpha \rightarrow 0$ without changing $A_0$ and $k$,
\begin{eqnarray}
	&&\textcolor{blue}{|\psi|^2} = A_0^2 \left[ \frac{\sin^2 (k\sin\alpha)x}{\sin\alpha^2} + \beta^2 k^2 y^2 \cos^2(k\sin\alpha)x \right]
	\nonumber\\
	&& \hspace{0.15in} \rightarrow A_0^2\left( k^2 x^2 + \beta^2 k^2 y^2 \right)
\end{eqnarray}
and
\begin{eqnarray}
	&&\Phi = 2n\pi + \left[(k \cos\alpha) z - \omega t \right] - \arctan\left(\frac{\beta \eta}{\tan \xi} \right)
	\nonumber\\
	&& \hspace{0.15in} \rightarrow 2n\pi + (kz - \omega t) - \arctan\left(\beta y/ x\right).
	\label{eq:limit}
\end{eqnarray}

Set $\beta = 1$ and represent Eq. (\ref{eq:limit}) in cylindrical coordinates, i.e. $(r, \phi, z)$ with $r^2 = x^2 + y^2, \phi = \arctan(y/x), z = z$,
\begin{eqnarray}
	\psi(r, \phi, z) = A_0 kr e^{i(k z - \omega t - \phi)}.
	\label{eq:single_vortex}
\end{eqnarray}
Eq. (\ref{eq:single_vortex}) characterizes an isolated skew-dislocation \cite{Ber73} of ``strength'' $m = 1$.

Having established the method to find the equation for a skew-dislocation by mixing two primary waves and performing a limiting process, Nye and Berry \cite{Ber73} claimed that these field expressions can be guessed \emph{a priori}. Therefore we need only generalize the present complex wave function $\psi$ we already have and keep they still satisfy the wave equation Eq. (\ref{eq:wave}). By this, we shall interpret the yielded functions as representing various kinds of dislocations, namely vortices.

In this perspective, Eq. (\ref{eq:single_vortex}) can be extended to the form
\begin{eqnarray}
	\psi = \left[ Ar^m + \left( \frac{B}{r^m} \right)\right] e^{i(kz - \omega t \pm m \phi)},
	\label{eq:vortex_m}
\end{eqnarray}
which still complies with Eq. (\ref{eq:wave}). Eq. (\ref{eq:vortex_m}) describes vortices with strength, or more precisely, topological charge, equals $m$. To define the topological charge, we consider a closed curve $C$ in the $(\bar{r}, t)$-space and perform the following steps:
\begin{enumerate}
	\item Around the curve $C$ the phase angle $\Phi$ may undergo a change of $2n \pi$, with $n \in {\cal Z}$ and $n \neq 0$.
	\item Shrink the closed curve $C$ to an arbitrarily small loop without changing $n$.
	\item If such a curve $C$ can be found, then $C$ is claimed to enclose a singularity because $\Phi$ varies infinitely fast 
	around the center point.
	\item The smoothness of the function $\psi$ implies that this scenario can only happen at points where $\psi = 0$, where $\Phi$ is not well-defined.
\end{enumerate}
A winding number $S_C$, characterizing the strength of this singularity, is defined as 
\begin{eqnarray}
	S_C = \frac{1}{2 \pi} \oint_C d \Phi = \frac{1}{2 \pi} \oint_C \nabla \Phi \cdot d \bar{r}
\end{eqnarray}
where $C$ is a contour enclosing the singularity.

\section*{Appendix II: 2-D Fourier Transformation of Vortex Beam}
To compute the counterpart in frequency domain of the field $U(r, \phi, 0) = e^{i\phi}$, we recall the Fourier transformation pair
\begin{eqnarray}
	A(f_x, f_y, z) = \int_{-\infty}^{\infty} \int_{-\infty}^{\infty} U(x, y, z)
	e^{-i 2 \pi (f_x x + f_y y)} dx dy
	\nonumber\\
	U(x, y, z) = \int_{-\infty}^{\infty} \int_{-\infty}^{\infty} A(f_x, f_y, z)
	e^{i 2 \pi (f_x x + f_y y)} df_x df_y.
	\nonumber
\end{eqnarray}
Perform the following change of variable:
\begin{eqnarray}
	x = r\cos\phi & y = r\sin\phi & r \ge 0, 0 \le \phi \le 2\pi
	\nonumber\\
	f_x = \rho\cos\chi & f_y = \rho\sin\chi & \rho \ge 0, 0 \le \chi \le 2\pi
	\nonumber
\end{eqnarray}
Thus, we have
\begin{eqnarray}
	&&dx dy = r dr d\phi, \hspace{0.1in} df_x df_y = \rho d\rho d\chi,
	\nonumber\\
	&&xf_x + yf_y = r\rho \cos(\phi - \chi).
	\nonumber
\end{eqnarray}
To sum up, the 2-D Fourier transformation pair in cylindrical coordinate is represented by
\begin{eqnarray}
	A(\rho, \chi, z) = \int_{0}^{2\pi} \int_{0}^{\infty} U(r, \phi, z)
	e^{-i 2 \pi r \rho \cos(\phi - \chi)} r dr d\phi
	\nonumber\\
	U(r, \phi, z) = \int_{0}^{2\pi} \int_{0}^{\infty} A(\rho, \chi, z)
	e^{i 2 \pi r \rho \cos(\phi - \chi)} \rho d\rho d\chi.
	\nonumber
\end{eqnarray}

Therefore, one can compute ${\cal F} \{e^{i\phi}\}$ as follows:
\begin{eqnarray}
	&&A(\rho, \chi, 0) = \int_{0}^{2\pi} e^{i\phi} 
	\left(\int_{0}^{\infty} e^{-i2\pi \rho r \cos(\phi - \chi)} r dr\right) d\phi
	\nonumber\\
	&&\hspace{0.5in}= \int_{0}^{2\pi} \frac{-e^{i\phi}}{4 \pi^2 \rho^2 \cos^2(\phi - \chi)} d\phi
	\nonumber\\
	&&\hspace{0.5in}= \frac{1}{\pi^2 \rho^2} \int_{0}^{2\pi} \frac{-e^{i\phi} d\phi}{e^{i(\phi - \chi)} + e^{-i(\phi - \chi)}}
	\nonumber\\
	&&\hspace{0.5in}= \frac{ e^{i\chi} }{\pi^2 \rho^2} \int_{\chi}^{\chi + 2\pi}
	\frac{-e^{i\phi'} d\phi'}{e^{i\phi'} + e^{-i\phi'}},
	\hspace{0.1in} (\phi' = \phi - \chi)
	\nonumber\\
	&&\hspace{0.5in}= \frac{i e^{i \chi}}{\pi^2 \rho^2} \oint_C \frac{dz}{(z + z^{-1})^2}
	\nonumber\\
	&&\hspace{0.5in}= \frac{i e^{i \chi}}{\pi^2 \rho^2} \oint_C \frac{z^2 dz}{(z^2 + 1)^2},
\end{eqnarray}
where the last complex contour integration is performed counterclockwise along the boundary $C$ of unit circle centered at the origin. Since the integrand in the last equality has two poles of order $2$ located at $i$ and $-i$ (both are on $C$), respectively, the contour integration can only be defined by Cauchy principal value, i.e.
\begin{eqnarray}
	{\cal P} \oint_C \frac{z^2 dz}{(z^2 + 1)^2} = \lim_{\epsilon \rightarrow 0} \oint_{C_{\epsilon}} \frac{z^2 dz}{(z^2 + 1)^2},
	\label{eq:CPV}
\end{eqnarray}
where $C_{\epsilon}$ is a curve defined as Fig. \ref{fig:contour}.
% Unable to show figure?
%\begin{figure}[h]
%	\vskip 6 cm
%	\hskip 0.3 cm
%	\special{wmf: contour.pdf x=7 cm y=6 cm}
%	\caption{Contour of $C_{\epsilon}$.}
%	\label{fig:contour}
%\end{figure}
\begin{figure}
		\centering
		\includegraphics[width = .4\textwidth]{contour.jpg}
		\caption{Contour of $C_{\epsilon}$, which is formed by the boundary of the union of the unit circle centered at the origin and two circles with radius $\epsilon$ centered at $i, -i$, repectively.}
		\label{fig:contour}
\end{figure}
Note that $C_{\epsilon} \rightarrow C$ as $\epsilon \rightarrow 0$. The contour integration on $C_{\epsilon}$, on the other hand, can be evaluated by residue theorem.
\begin{eqnarray}
	\oint_{C_{\epsilon}} \frac{z^2}{(z^2 + 1)^2} = 2\pi i \left( {\rm Res}(f; i) + {\rm Res}(f; -i) \right),
	\label{eq:thm_residue}
\end{eqnarray}
with $f$ denoting the integrand in Eq. (\ref{eq:CPV}). By invoking the identity ${\rm Res}(f; a) = 1/(n-1)! \lim_{z \rightarrow a} d^n (z - a)^n f(z) /dz^n$ for a pole $a$ of order $n$, the residues can be computed:
\begin{eqnarray}
	{\rm Res}(f; i) = 1/8, & {\rm Res}(f; -i) = 3/8.
	\nonumber
\end{eqnarray}
Hence, Eq. (\ref{eq:thm_residue}) yields
\begin{eqnarray}
	A(\rho, \chi, 0) = \frac{- e^{i \chi}}{\pi \rho^2}. (?)
\end{eqnarray}

\section*{Appendix III: Paraxial Wave Eqation}
Given a monochromatic electromagnetic field $\tilde{U}(x, y, z) \exp(-i \omega t) = U(x, y, z)\exp[i (kz - \omega t)]$, we have known that it satisfies the Helmholtz equation
\begin{eqnarray}
	\left(\nabla^2 + k^2\right) \tilde{U}(x, y, z) = 0.
	\label{eq:helmholtz}
\end{eqnarray}
If we compute
\begin{eqnarray}
	\frac{\partial^2}{\partial z^2} U(x, y, z)e^{ikz} = e^{ikz}
	\left( \frac{\partial^2 U}{\partial z^2} + 2ik \frac{\partial U}{\partial z} - k^2 U \right),
	\nonumber
\end{eqnarray}
Then Eq. (\ref{eq:helmholtz}) becomes
\begin{eqnarray}
	\left(\frac{\partial^2}{\partial x^2} + \frac{\partial^2}{\partial y^2} + \frac{\partial^2}{\partial z^2} + 2ik \frac{\partial}{\partial z} \right) U(x, y, z) = 0
	\label{eq:helmholtz_2}
\end{eqnarray}
One can further simplify the equation by performing {\em the paraxial approximation}:
\begin{eqnarray}
	\left| \frac{\partial^2 U}{\partial z^2} \right| \ll \left| 2k \frac{\partial U}{\partial z} \right|,
	\label{eq:paraxial}
\end{eqnarray}
which can be interpreted physically that the variation along $z$-axis is so small that all of the light must travel nearly paralle to the $z$-axis. Therefore, Eq. (\ref{eq:helmholtz_2}) is reduced to
\begin{eqnarray}
	\left(\nabla_{\perp}^2 + 2ik \frac{\partial}{\partial z} \right) U(x, y, z) = 0.
	\label{eq:pwe}
\end{eqnarray}
Usually, laser beams satisfy the paraxial approximation (\ref{eq:paraxial}) very well, whence it is convenient to model them by Eq. (\ref{eq:pwe}).

\section*{Appendix IV: Fast Fourier Transform}
Here we introduce a powerful algorithm to evaluate a Fourier transform numerically. In the first step, one needs to converse the continuous time-domain (or, in our case, space-domain) function to a digital one. The corresponding transformation pair is called {\em digital Fourier transform} (DFT).

Let $U = U(x)$ be a single-variable function of space. In order to perform DFT suitably, the space function $U$ must have a bounded support, i.e. there is some finite number $X_0$ such that $U(x) = 0$ unless $|x| \leq X_0$. Otherwise, the function $U(x)$ must be {\em windowed}. Therefore, we may well suppose that $U(x) \neq 0$ only if $0 \leq x \leq X_0$. Now pick $N$ equispaced sample points $x = 0, X_s, 2X_s, \dots, (N-1)X_s$, where $X_s = X_0/N$, and then we can represent the sampled function $U_{\delta}$ by
\begin{eqnarray}
	&&U_{\delta} = U(x) \cdot \sum_{n = 0}^{N-1} \delta(x - n X_s)
	\nonumber\\
	&&\hspace{0.2in} = \sum_{n = 0}^{N-1} U(n X_s) \delta(x - n X_s),
\end{eqnarray}
with $\delta$ being the Dirac delta function. The corresponding discrete-time Fourier transform is given by
\begin{eqnarray}
	A_{\delta}(\nu) = \int_{-\infty}^{\infty} U_{\delta}(x) e^{-i \nu x} dx
	\nonumber\\
	\hspace{0.3in} = \sum_{n = 0}^{N - 1} U(n X_s) e^{-i \nu n X_s}.
\end{eqnarray}
Our next step is to discretize the spectrum as well, which is equivalent to making $U_{\delta}$ a periodic function in the space-domain. Let $U'(x)$ be such a periodic function extended from $U_{\delta}$ with period $X_0$, i.e.
\begin{eqnarray}
	U'(x) = U_{\delta}(x) * \sum_{m = -\infty}^{\infty} \delta(x - m X_0),
\end{eqnarray}
where $*$ denotes the convolution. We have the corresponding spectrum
\begin{eqnarray}
	&& A'(\nu) = A_{\delta} \cdot \frac{2\pi}{X_0} \sum_{m = -\infty}^{\infty} \delta(\nu - \frac{2\pi m}{X_0})
	\nonumber\\
	&&= \frac{2\pi}{X_0} \sum_{m = -\infty}^{\infty} \left(\sum_{n = 0}^{N - 1}
		U(n \frac{X_0}{N}) e^{-i 2\pi m n/ N}\right) \delta(\nu - \frac{2\pi m}{X_0}).
	\nonumber
\end{eqnarray}
Define $U[n] = U(n X_0 / N)$ and
\begin{eqnarray}
	A[m] = \sum_{n = 0}^{N - 1} U[n] e^{-i 2\pi m n/ N}.
	\label{eq:DFT}
\end{eqnarray}
Eq. (\ref{eq:DFT}) is the definition of digital Fourier transform. Note that we have the relation
\begin{eqnarray}
	&&A(\frac{2 \pi m}{X_0}) = \frac{2\pi}{X_0} \sum_{k = -\infty}^{\infty} A[k]
		\delta(\frac{2 \pi}{X_0} (m - k))
	\nonumber\\
	&&\hspace{0.5in}=  \frac{2\pi}{X_0} A[m] \delta(0).
\end{eqnarray}
In order to obtain the expression for inverse digital Fourier transform, we recall the identity
\begin{eqnarray}
	\sum_{k = 0}^{N - 1} e^{-i 2 \pi k(n - m)/N} = N \delta(n - m),
\end{eqnarray}
from which and Eq. (\ref{eq:DFT}) we will end up with
\begin{eqnarray}
	&&\sum_{k = 0}^{N - 1} A[k] e^{i 2 \pi mk/N} 
	\nonumber\\
	&&\hspace{0.3in} = \sum_{k = 0}^{N - 1} \sum_{n = 0}^{N - 1} U[n] e^{-i 2 \pi k(n - m)/N}
	\nonumber\\
	&&\hspace{0.3in} = N \sum_{n = 0}^{N - 1} U[n] \delta(n - m) = N U[m].
\end{eqnarray}
To sum up, the definitions of DFT and inverse DFT are obtained from the known continuous Fourier transform and represented as
\begin{eqnarray}
	&&A[m] = \sum_{n = 0}^{N - 1} U[n] e^{-i 2\pi m n/ N}
	\nonumber\\
	&&U[n] = \frac{1}{N} \sum_{m = 0}^{N - 1} A[m] e^{i 2 \pi mn/N}.
	\label{eq:DFT_pairs}
\end{eqnarray}
The definition shown in Eq. (\ref{eq:DFT_pairs}) also corresponds to that of MATLAB, so there is no need to amend equations while working on the codes.